move theorems away from Ott file

examples/compute/src/theory/birScript.sml
@@ -106,19 +106,6 @@ Definition birF_def:
   birF = BVal_Imm (Imm1 0w)
 End
 
-(* Correction Theorems of boolean functions *)
-Theorem bool2b_T_eq_birT:
-  BVal_Imm (bool2b T) = birT
-Proof
-  rw [bool2b_def, bool2w_def, birT_def]
-QED
-
-Theorem bool2b_F_eq_birF:
-  BVal_Imm (bool2b F) = birF
-Proof
-  rw [bool2b_def, bool2w_def, birF_def]
-QED
-
 (* Utility functions *)
 Definition bir_dest_bool_val_def:
   (bir_dest_bool_val (BVal_Imm (Imm1 w)) = SOME (w = 1w)) /\
@@ -156,64 +143,6 @@ End
 Definition bir_env_update_def:
   bir_env_update ((BEnv env):bir_var_environment_t) (BVar id) v = BEnv ((id =+ SOME v) env)
 End
-
-Theorem bir_env_lookup_empty:
-  !var v. ~(bir_env_lookup_rel bir_empty_env var v)
-Proof
-  Cases_on `var` >>
-  rw [bir_empty_env_def, bir_env_lookup_rel_def]
-QED
-
-Theorem bir_env_lookup_rel_update:
-  !env var v. bir_env_lookup_rel (bir_env_update env var v) var v 
-Proof
-  Cases_on `var` >> Cases_on `env` >>
-  rw [bir_env_update_def, bir_env_lookup_rel_def]
-QED
-
-Theorem bir_env_lookup_update:
-  !env var v. bir_env_lookup (bir_env_update env var v) var = SOME v 
-Proof
-  rpt gen_tac >>
-  Cases_on `var` >> Cases_on `env` >>
-  rw [bir_env_update_def, bir_env_lookup_def]
-QED
-
-Theorem bir_env_lookup_update_neq:
-  !env var1 var2 v. 
-    var1 <> var2 ==>
-      bir_env_lookup (bir_env_update env var1 v) var2 = bir_env_lookup env var2
-Proof
-  Cases_on `var1` >> Cases_on `var2` >>
-  rw [fetch "-" "bir_var_t_11"] >>
-  Cases_on `env` >>
-  simp [bir_env_update_def] >>
-  rw [bir_env_lookup_def] >>
-  EVAL_TAC >>
-  metis_tac []
-QED
-
-(* Lookup and relation are the same *)
-Theorem bir_env_lookup_eq_rel:
-  !env var v. bir_env_lookup_rel env var v <=> bir_env_lookup env var = SOME v
-Proof
-  rpt strip_tac >>
-  Cases_on `env` >>
-  Cases_on `var` >>
-    rw [bir_env_lookup_def, bir_env_lookup_rel_def]
-QED
-
-
-(* Injective *)
-Theorem bir_env_lookup_rel_inj:
-  !env var v1 v2.
-    bir_env_lookup_rel env var v1 ==>
-    bir_env_lookup_rel env var v2 ==>
-    v1 = v2
-Proof
-  Cases_on `env` >> Cases_on `var` >>
-    simp [bir_env_lookup_rel_def]
-QED
 
 (* --------- Typing ------- *)
 
@@ -356,384 +285,6 @@ Inductive type_of_bir_exp:
 ( ( type_of_bir_exp env (BExp_Store bir_exp1 bir_exp2 BEnd_LittleEndian bir_exp3) (BType_Mem bir_immtype1 bir_immtype2) )))
 End
 
-Definition is_exp_well_typed_def:
-  is_exp_well_typed env exp = ?ty. type_of_bir_exp env exp ty
-End
-
-(* 1 bit values are booleans *)
-Theorem bit1_is_boolean:
-  !v. type_of_bir_val v = (BType_Imm Bit1) ==> (v = birT \/ v = birF)
-Proof
-  Cases_on `v` >>
-    Cases_on `b` >>
-      rw [birT_def, birF_def, type_of_bir_val_def, type_of_bir_imm_def] >>
-      Cases_on `c` >>
-        fs [dimword_1]
-QED
-
-(* Gets the operator for a given binary operation *)
-Definition bir_binexp_get_oper_def:
-  (bir_binexp_get_oper BIExp_And = word_and) /\
-  (bir_binexp_get_oper BIExp_Plus = word_add)
-End
-(* Evaluates a binary expression of two immediates *)
-Inductive bir_eval_binexp_imm:
-  (!binexp w1 w2. 
-    bir_eval_binexp_imm binexp (Imm1 w1) (Imm1 w2) (Imm1 ((bir_binexp_get_oper binexp) w1 w2))) /\
-  (!binexp w1 w2. 
-    bir_eval_binexp_imm binexp (Imm8 w1) (Imm8 w2) (Imm8 ((bir_binexp_get_oper binexp) w1 w2))) /\
-  (!binexp w1 w2. 
-    bir_eval_binexp_imm binexp (Imm16 w1) (Imm16 w2) (Imm16 ((bir_binexp_get_oper binexp) w1 w2))) /\
-  (!binexp w1 w2. 
-    bir_eval_binexp_imm binexp (Imm32 w1) (Imm32 w2) (Imm32 ((bir_binexp_get_oper binexp) w1 w2))) /\
-  (!binexp w1 w2. 
-    bir_eval_binexp_imm binexp (Imm64 w1) (Imm64 w2) (Imm64 ((bir_binexp_get_oper binexp) w1 w2))) /\
-  (!binexp w1 w2. 
-    bir_eval_binexp_imm binexp (Imm128 w1) (Imm128 w2) (Imm128 ((bir_binexp_get_oper binexp) w1 w2)))
-End
-
-(* Evaluates a general binary expression with values as parameters *)
-Definition bir_eval_binexp_def:
-  (bir_eval_binexp binexp (BVal_Imm imm1) (BVal_Imm imm2) (BVal_Imm imm) =
-    (bir_eval_binexp_imm binexp imm1 imm2 imm)) /\
-  (bir_eval_binexp _ _ _ _ = F)
-End
-
-(* Computes a binary expression of two immediates *)
-Definition bir_compute_binexp_imm_def:
-  (bir_compute_binexp_imm BIExp_And (Imm1 w1) (Imm1 w2) = SOME (Imm1 (word_and w1 w2))) /\
-  (bir_compute_binexp_imm BIExp_And (Imm8 w1) (Imm8 w2) = SOME (Imm8 (word_and w1 w2))) /\
-  (bir_compute_binexp_imm BIExp_And (Imm16 w1) (Imm16 w2) = SOME (Imm16 (word_and w1 w2))) /\
-  (bir_compute_binexp_imm BIExp_And (Imm32 w1) (Imm32 w2) = SOME (Imm32 (word_and w1 w2))) /\
-  (bir_compute_binexp_imm BIExp_And (Imm64 w1) (Imm64 w2) = SOME (Imm64 (word_and w1 w2))) /\
-  (bir_compute_binexp_imm BIExp_And (Imm128 w1) (Imm128 w2) = SOME (Imm128 (word_and w1 w2))) /\
-  (bir_compute_binexp_imm BIExp_Plus (Imm1 w1) (Imm1 w2) = SOME (Imm1 (word_add w1 w2))) /\
-  (bir_compute_binexp_imm BIExp_Plus (Imm8 w1) (Imm8 w2) = SOME (Imm8 (word_add w1 w2))) /\
-  (bir_compute_binexp_imm BIExp_Plus (Imm16 w1) (Imm16 w2) = SOME (Imm16 (word_add w1 w2))) /\
-  (bir_compute_binexp_imm BIExp_Plus (Imm32 w1) (Imm32 w2) = SOME (Imm32 (word_add w1 w2))) /\
-  (bir_compute_binexp_imm BIExp_Plus (Imm64 w1) (Imm64 w2) = SOME (Imm64 (word_add w1 w2))) /\
-  (bir_compute_binexp_imm BIExp_Plus (Imm128 w1) (Imm128 w2) = SOME (Imm128 (word_add w1 w2))) /\
-  (bir_compute_binexp_imm binexp _ _ = NONE)
-End
-
-
-(* Computes a general binary expression with values as parameters *)
-Definition bir_compute_binexp_def:
-  (bir_compute_binexp binexp (SOME (BVal_Imm imm1)) (SOME (BVal_Imm imm2)) =
-    val_from_imm_option (bir_compute_binexp_imm binexp imm1 imm2)) /\
-  (bir_compute_binexp _ _ _ = NONE)
-End
-
-(* Eval and compute are similar *)
-Theorem bir_eval_binexp_eq_compute_binexp:
-  !binexp v1 v2 v. bir_eval_binexp binexp v1 v2 v <=> 
-    bir_compute_binexp binexp (SOME v1) (SOME v2) = SOME v
-Proof
-  Cases_on `binexp` >>
-  Cases_on `v1` >> Cases_on `v2` >> Cases_on `v` >>
-    rw [bir_eval_binexp_def, bir_compute_binexp_def] >>
-    rw [bir_eval_binexp_imm_cases, bir_compute_binexp_imm_def] >>
-    Cases_on `b` >> Cases_on `b'` >> Cases_on `b''` >>
-      rw [bir_compute_binexp_imm_def, fetch "-" "bir_imm_t_nchotomy", bir_binexp_get_oper_def] >>
-      rw [val_from_imm_option_def] >>
-      metis_tac []
-QED
-
-
-(* If the operands are typed, then the expression evaluates *)
-Theorem type_of_bir_val_imp_bir_eval_binexp:
-  !binexp v1 v2 ty.
-    ((type_of_bir_val v1 = BType_Imm ty) /\ (type_of_bir_val v2 = BType_Imm ty)) ==>
-    ?v. bir_eval_binexp binexp v1 v2 v
-Proof
-  Cases_on `binexp` >>
-  Cases_on `v1` >> Cases_on `v2` >>
-  Cases_on `b` >> Cases_on `b'` >>
-    rw [bir_eval_binexp_eq_compute_binexp] >>
-    rw [bir_compute_binexp_def, bir_compute_binexp_imm_def] >>
-    rw [val_from_imm_option_def] >>
-    fs [type_of_bir_val_def, type_of_bir_imm_def]
-QED
-
-
-(* Type conservation Theorem *)
-Theorem bir_eval_binexp_keep_type:
-  !binexp v1 v2 v ty.
-    bir_eval_binexp binexp v1 v2 v ==>
-    ((type_of_bir_val v1 = ty /\ type_of_bir_val v2 = ty) <=>
-      type_of_bir_val v = ty)
-Proof
-  Cases_on `v1` >> Cases_on `v2` >> Cases_on `v` >>
-  Cases_on `b` >> Cases_on `b'` >> Cases_on `b''` >>
-    rw [type_of_bir_val_def, bir_eval_binexp_def, type_of_bir_imm_def, bir_eval_binexp_imm_cases]
-QED
-
-(* Gets the operator for a given unary operation *)
-Definition bir_unaryexp_get_oper_def:
-  (bir_unaryexp_get_oper BIExp_Not = word_1comp) /\
-  (bir_unaryexp_get_oper BIExp_ChangeSign = word_2comp)
-End
-
-
-(* Evaluates a binary expression of an immediate *)
-Inductive bir_eval_unaryexp_imm:
-  (!unaryexp w1. 
-    bir_eval_unaryexp_imm unaryexp (Imm1 w1) (Imm1 ((bir_unaryexp_get_oper unaryexp) w1))) /\
-  (!unaryexp w1. 
-    bir_eval_unaryexp_imm unaryexp (Imm8 w1) (Imm8 ((bir_unaryexp_get_oper unaryexp) w1))) /\
-  (!unaryexp w1. 
-    bir_eval_unaryexp_imm unaryexp (Imm16 w1) (Imm16 ((bir_unaryexp_get_oper unaryexp) w1))) /\
-  (!unaryexp w1. 
-    bir_eval_unaryexp_imm unaryexp (Imm32 w1) (Imm32 ((bir_unaryexp_get_oper unaryexp) w1))) /\
-  (!unaryexp w1. 
-    bir_eval_unaryexp_imm unaryexp (Imm64 w1) (Imm64 ((bir_unaryexp_get_oper unaryexp) w1))) /\
-  (!unaryexp w1. 
-    bir_eval_unaryexp_imm unaryexp (Imm128 w1) (Imm128 ((bir_unaryexp_get_oper unaryexp) w1)))
-End
-
-
-(* Evaluates a general unary expression with values as parameters *)
-Definition bir_eval_unaryexp_def:
-  (bir_eval_unaryexp unaryexp (BVal_Imm imm1) (BVal_Imm imm) =
-    (bir_eval_unaryexp_imm unaryexp imm1 imm)) /\
-  (bir_eval_unaryexp _ _ _ = F)
-End
-
-(* Computes a binary expression of an immediate *)
-Definition bir_compute_unaryexp_imm_def:
-  (bir_compute_unaryexp_imm BIExp_Not (Imm1 w1) = SOME (Imm1 (word_1comp w1))) /\
-  (bir_compute_unaryexp_imm BIExp_Not (Imm8 w1) = SOME (Imm8 (word_1comp w1))) /\
-  (bir_compute_unaryexp_imm BIExp_Not (Imm16 w1) = SOME (Imm16 (word_1comp w1))) /\
-  (bir_compute_unaryexp_imm BIExp_Not (Imm32 w1) = SOME (Imm32 (word_1comp w1))) /\
-  (bir_compute_unaryexp_imm BIExp_Not (Imm64 w1) = SOME (Imm64 (word_1comp w1))) /\
-  (bir_compute_unaryexp_imm BIExp_Not (Imm128 w1) = SOME (Imm128 (word_1comp w1))) /\
-  (bir_compute_unaryexp_imm BIExp_ChangeSign (Imm1 w1) = SOME (Imm1 (word_2comp w1))) /\
-  (bir_compute_unaryexp_imm BIExp_ChangeSign (Imm8 w1) = SOME (Imm8 (word_2comp w1))) /\
-  (bir_compute_unaryexp_imm BIExp_ChangeSign (Imm16 w1) = SOME (Imm16 (word_2comp w1))) /\
-  (bir_compute_unaryexp_imm BIExp_ChangeSign (Imm32 w1) = SOME (Imm32 (word_2comp w1))) /\
-  (bir_compute_unaryexp_imm BIExp_ChangeSign (Imm64 w1) = SOME (Imm64 (word_2comp w1))) /\
-  (bir_compute_unaryexp_imm BIExp_ChangeSign (Imm128 w1) = SOME (Imm128 (word_2comp w1)))
-End
-
-(* Computes Unary expression *)
-Definition bir_compute_unaryexp_def:
-  (bir_compute_unaryexp unaryexp (SOME (BVal_Imm imm1)) = 
-    val_from_imm_option (bir_compute_unaryexp_imm unaryexp imm1)) /\
-  (bir_compute_unaryexp _ _ = NONE)
-End
-
-(* Eval and Compute are similar *)
-Theorem bir_eval_unaryexp_eq_compute_unaryexp:
-  !unaryexp v1 v. bir_eval_unaryexp unaryexp v1 v <=> 
-    bir_compute_unaryexp unaryexp (SOME v1) = SOME v
-Proof
-  Cases_on `unaryexp` >>
-  Cases_on `v1` >> Cases_on `v` >>
-    rw [bir_eval_unaryexp_def, bir_compute_unaryexp_def] >>
-    rw [bir_eval_unaryexp_imm_cases, bir_compute_unaryexp_imm_def] >>
-    Cases_on `b` >> Cases_on `b'` >>
-      rw [bir_compute_unaryexp_imm_def, fetch "-" "bir_imm_t_nchotomy", bir_unaryexp_get_oper_def] >>
-      rw [val_from_imm_option_def] >>
-      metis_tac []
-QED
-
-
-(* Unary_exp always evaluates *)
-Theorem type_of_bir_val_imp_bir_eval_unaryexp:
-  !unaryexp v ty.
-    (type_of_bir_val v = BType_Imm ty) ==>
-    ?v'. bir_eval_unaryexp unaryexp v v'
-Proof
-  Cases_on `unaryexp` >>
-  Cases_on `v` >>
-  Cases_on `b` >>
-    rw [bir_eval_unaryexp_eq_compute_unaryexp, type_of_bir_val_def] >>
-    rw [bir_compute_unaryexp_def, bir_compute_unaryexp_imm_def] >>
-    rw [val_from_imm_option_def] >>
-    fs [type_of_bir_val_def, type_of_bir_imm_def]
-QED
-
-(* Type conservation theorem *)
-Theorem bir_eval_unaryexp_keep_type:
-  !unaryexp v1 v2 ty.
-    bir_eval_unaryexp unaryexp v1 v2 ==>
-    (type_of_bir_val v1 = type_of_bir_val v2)
-Proof
-  Cases_on `v1` >> Cases_on `v2` >>
-  Cases_on `b` >> Cases_on `b'` >>
-    rw [type_of_bir_val_def, bir_eval_unaryexp_def, type_of_bir_imm_def, bir_eval_unaryexp_imm_cases]
-QED
-
-(* Gets the operator for a given binary predicate *)
-Definition bir_binpred_get_oper_def:
-  (bir_binpred_get_oper BIExp_Equal = $=) /\
-  (bir_binpred_get_oper BIExp_LessThan = word_lo)
-End
-
-
-(* Evaluates a binary predicate of two immediates *)
-Inductive bir_eval_binpred_imm:
-  (!binpred w1 w2. 
-    bir_eval_binpred_imm binpred (Imm1 w1) (Imm1 w2) ((bir_binpred_get_oper binpred) w1 w2)) /\
-  (!binpred w1 w2. 
-    bir_eval_binpred_imm binpred (Imm8 w1) (Imm8 w2) ((bir_binpred_get_oper binpred) w1 w2)) /\
-  (!binpred w1 w2. 
-    bir_eval_binpred_imm binpred (Imm16 w1) (Imm16 w2) ((bir_binpred_get_oper binpred) w1 w2)) /\
-  (!binpred w1 w2. 
-    bir_eval_binpred_imm binpred (Imm32 w1) (Imm32 w2) ((bir_binpred_get_oper binpred) w1 w2)) /\
-  (!binpred w1 w2. 
-    bir_eval_binpred_imm binpred (Imm64 w1) (Imm64 w2) ((bir_binpred_get_oper binpred) w1 w2)) /\
-  (!binpred w1 w2. 
-    bir_eval_binpred_imm binpred (Imm128 w1) (Imm128 w2) ((bir_binpred_get_oper binpred) w1 w2))
-End
-
-
-(* Evaluates a general binary predicate with values as parameters *)
-Inductive bir_eval_binpred:
-  (!binpred imm1 imm2 b. 
-    (bir_eval_binpred_imm binpred imm1 imm2 b) ==>
-    (bir_eval_binpred binpred (BVal_Imm imm1) (BVal_Imm imm2) (BVal_Imm (bool2b b))))
-End
-
-(* Computes a binary predicate of two immediates *)
-Definition bir_compute_binpred_imm_def:
-  (bir_compute_binpred_imm BIExp_Equal (Imm1 w1) (Imm1 w2) = $= w1 w2) /\
-  (bir_compute_binpred_imm BIExp_Equal (Imm8 w1) (Imm8 w2) = $= w1 w2) /\
-  (bir_compute_binpred_imm BIExp_Equal (Imm16 w1) (Imm16 w2) = $= w1 w2) /\
-  (bir_compute_binpred_imm BIExp_Equal (Imm32 w1) (Imm32 w2) = $= w1 w2) /\
-  (bir_compute_binpred_imm BIExp_Equal (Imm64 w1) (Imm64 w2) = $= w1 w2) /\
-  (bir_compute_binpred_imm BIExp_Equal (Imm128 w1) (Imm128 w2) = $= w1 w2) /\
-  (bir_compute_binpred_imm BIExp_LessThan (Imm1 w1) (Imm1 w2) = word_lo w1 w2) /\
-  (bir_compute_binpred_imm BIExp_LessThan (Imm8 w1) (Imm8 w2) = word_lo w1 w2) /\
-  (bir_compute_binpred_imm BIExp_LessThan (Imm16 w1) (Imm16 w2) = word_lo w1 w2) /\
-  (bir_compute_binpred_imm BIExp_LessThan (Imm32 w1) (Imm32 w2) = word_lo w1 w2) /\
-  (bir_compute_binpred_imm BIExp_LessThan (Imm64 w1) (Imm64 w2) = word_lo w1 w2) /\
-  (bir_compute_binpred_imm BIExp_LessThan (Imm128 w1) (Imm128 w2) = word_lo w1 w2) /\
-  (bir_compute_binpred_imm binpred _ _ = F)
-End
-
-
-(* Computes a general binary predicate with values as parameters *)
-Definition bir_compute_binpred_def:
-  (bir_compute_binpred binpred (SOME (BVal_Imm imm1)) (SOME (BVal_Imm imm2)) =
-    SOME (BVal_Imm (bool2b (bir_compute_binpred_imm binpred imm1 imm2)))) /\
-  (bir_compute_binpred _ _ _ = NONE)
-End
-
-Theorem bir_eval_binpred_imp_compute_binpred:
-  !binpred v1 v2 v. bir_eval_binpred binpred v1 v2 v ==> 
-    bir_compute_binpred binpred (SOME v1) (SOME v2) = SOME v
-Proof
-  Cases_on `binpred` >>
-  Cases_on `v1` >> Cases_on `v2` >> Cases_on `v` >>
-    rw [bir_eval_binpred_cases, bir_compute_binpred_def] >>
-    rw [bir_eval_binpred_imm_cases, bir_compute_binpred_imm_def] >>
-    Cases_on `b` >> Cases_on `b'` >>
-      rw [bool2b_def, bool2w_def, bir_compute_binpred_imm_def, fetch "-" "bir_imm_t_nchotomy"] >>
-      fs [bir_eval_binpred_imm_cases, bir_binpred_get_oper_def] >>
-      metis_tac []
-QED
-
-(* If the term is well typed, then eval and compute are the same *)
-Theorem well_typed_bir_eval_binpred_eq_compute_binpred:
-  !binpred v1 v2 v. 
-    (type_of_bir_val v1 = type_of_bir_val v2) ==>
-  ( bir_eval_binpred binpred v1 v2 v <=> 
-    bir_compute_binpred binpred (SOME v1) (SOME v2) = SOME v)
-Proof
-  Cases_on `binpred` >>
-  Cases_on `v1` >> Cases_on `v2` >> Cases_on `v` >>
-  rw [bir_eval_binpred_cases, bir_compute_binpred_def] >>
-  rw [bir_eval_binpred_imm_cases, bir_compute_binpred_imm_def] >>
-  Cases_on `b` >> Cases_on `b'` >>
-    rw [bool2b_def, bool2w_def, bir_compute_binpred_imm_def, fetch "-" "bir_imm_t_nchotomy"] >>
-    fs [bir_eval_binpred_imm_cases, type_of_bir_val_def, type_of_bir_imm_def,
-      bir_binpred_get_oper_def] >>
-    metis_tac []
-QED
-
-
-(* If the operands are typed, then the expression evaluates *)
-Theorem type_of_bir_val_imp_bir_eval_binpred:
-  !binpred v1 v2 ty.
-    ((type_of_bir_val v1 = BType_Imm ty) /\ (type_of_bir_val v2 = BType_Imm ty)) ==>
-    ?v. bir_eval_binpred binpred v1 v2 v
-Proof
-  Cases_on `v1` >> Cases_on `v2` >>
-  Cases_on `b` >> Cases_on `b'` >>
-    rw [well_typed_bir_eval_binpred_eq_compute_binpred] >>
-    rw [bir_compute_binpred_def, bir_compute_binpred_imm_def] >>
-    fs [type_of_bir_val_def, type_of_bir_imm_def]
-QED
-
-
-(* Type conservation theorem *)
-Theorem bir_eval_binpred_correct_type:
-  !binpred v1 v2 v ty.
-    bir_eval_binpred binpred v1 v2 v ==>
-    ((type_of_bir_val v1 = type_of_bir_val v2) /\ type_of_bir_val v = (BType_Imm Bit1))
-Proof
-  Cases_on `v1` >> Cases_on `v2` >> Cases_on `v` >>
-  Cases_on `b` >> Cases_on `b'` >> Cases_on `b''` >>
-    rw [type_of_bir_val_def, bir_eval_binpred_cases, type_of_bir_imm_def, bir_eval_binpred_imm_cases, bool2b_def]
-QED
-
-(* Evaluates a general ifthenelse expression with values as parameters *)
-Inductive bir_eval_ifthenelse:
-[~BExp_IfThenElseT:]
-  bir_eval_ifthenelse birT (v1:bir_val_t) (v2:bir_val_t) v1 
-
-[~BExp_IfThenElseF:]
-  bir_eval_ifthenelse birF v1 v2 v2
-End
-
-(* Computes an ifthenelse expression of two values *)
-Definition bir_compute_ifthenelse_def:
-  bir_compute_ifthenelse b v1 v2 = 
-    if b = SOME birT then v1 
-    else if b = SOME birF then v2
-    else NONE
-End
-(* Eval and compute are similar *)
-Theorem bir_eval_ifthenelse_eq_compute_ifthenelse:
-  !v (v1:bir_val_t) (v2:bir_val_t) (v3:bir_val_t).
-  (bir_eval_ifthenelse v v1 v2 v3 <=>
-    bir_compute_ifthenelse (SOME v) (SOME v1) (SOME v2) = SOME v3)
-Proof
-  Cases_on `v` >> Cases_on `v1` >> Cases_on `v2` >> Cases_on `v3` >>
-  rw [bir_eval_ifthenelse_cases, bir_compute_ifthenelse_def, birT_def, birF_def] >>
-    metis_tac []
-QED
-
-(* If the condition is typed, then the expression evaluates *)
-Theorem type_of_bir_val_imp_bir_eval_ifthenelse:
-  !v v1 v2.
-    (type_of_bir_val v = (BType_Imm Bit1)) ==>
-    ?v3. bir_eval_ifthenelse v v1 v2 v3
-Proof
-  rw [bir_eval_ifthenelse_eq_compute_ifthenelse] >>
-  Cases_on `v` >| [
-    Cases_on `b` >>
-    Cases_on `c` >>
-      metis_tac [bir_compute_ifthenelse_def, bit1_is_boolean],
-
-    fs [type_of_bir_val_def]
-    ]
-QED
-
-(* Type conservation Theorem *)
-Theorem bir_eval_ifthenelse_keep_type:
-  !v v1 v2 v3 ty.
-    bir_eval_ifthenelse v v1 v2 v3 ==>
-    (type_of_bir_val v1 = ty /\ type_of_bir_val v2 = ty) ==>
-    (type_of_bir_val v = (BType_Imm Bit1) <=> type_of_bir_val v3 = ty)
-Proof
-  Cases_on `v` >> Cases_on `v1` >> Cases_on `v2` >> Cases_on `v3` >>
-  Cases_on `b` >> Cases_on `b'` >> Cases_on `b''` >> Cases_on `b'''` >>
-  rw [type_of_bir_val_def, bir_eval_ifthenelse_cases, type_of_bir_imm_def,
-    birT_def, birF_def]
-QED
-
 (* Number to Bitstring *)
 Definition n2bs_def:
   (n2bs n Bit1   = Imm1   (n2w n)) /\
@@ -748,7 +299,6 @@ End
 Definition v2bs_def:
   v2bs v s = n2bs (v2n v) s
 End
-
 
 (* Immediate to number *)
 Definition b2n_def:
@@ -785,11 +335,105 @@ Definition bitstring_split_def:
   bitstring_split n bs = bitstring_split_aux n [] bs
 End
 
+Definition is_exp_well_typed_def:
+  is_exp_well_typed env exp = ?ty. type_of_bir_exp env exp ty
+End
 
-(* ------------------------------------------ *)
-(* ------------------ LOAD ------------------ *)
-(* ------------------------------------------ *)
+(* Gets the operator for a given binary operation *)
+Definition bir_binexp_get_oper_def:
+  (bir_binexp_get_oper BIExp_And = word_and) /\
+  (bir_binexp_get_oper BIExp_Plus = word_add)
+End
 
+(* Evaluates a binary expression of two immediates *)
+Inductive bir_eval_binexp_imm:
+  (!binexp w1 w2. 
+    bir_eval_binexp_imm binexp (Imm1 w1) (Imm1 w2) (Imm1 ((bir_binexp_get_oper binexp) w1 w2))) /\
+  (!binexp w1 w2. 
+    bir_eval_binexp_imm binexp (Imm8 w1) (Imm8 w2) (Imm8 ((bir_binexp_get_oper binexp) w1 w2))) /\
+  (!binexp w1 w2. 
+    bir_eval_binexp_imm binexp (Imm16 w1) (Imm16 w2) (Imm16 ((bir_binexp_get_oper binexp) w1 w2))) /\
+  (!binexp w1 w2. 
+    bir_eval_binexp_imm binexp (Imm32 w1) (Imm32 w2) (Imm32 ((bir_binexp_get_oper binexp) w1 w2))) /\
+  (!binexp w1 w2. 
+    bir_eval_binexp_imm binexp (Imm64 w1) (Imm64 w2) (Imm64 ((bir_binexp_get_oper binexp) w1 w2))) /\
+  (!binexp w1 w2. 
+    bir_eval_binexp_imm binexp (Imm128 w1) (Imm128 w2) (Imm128 ((bir_binexp_get_oper binexp) w1 w2)))
+End
+
+(* Evaluates a general binary expression with values as parameters *)
+Definition bir_eval_binexp_def:
+  (bir_eval_binexp binexp (BVal_Imm imm1) (BVal_Imm imm2) (BVal_Imm imm) =
+    (bir_eval_binexp_imm binexp imm1 imm2 imm)) /\
+  (bir_eval_binexp _ _ _ _ = F)
+End
+
+(* Gets the operator for a given unary operation *)
+Definition bir_unaryexp_get_oper_def:
+  (bir_unaryexp_get_oper BIExp_Not = word_1comp) /\
+  (bir_unaryexp_get_oper BIExp_ChangeSign = word_2comp)
+End
+
+(* Evaluates a binary expression of an immediate *)
+Inductive bir_eval_unaryexp_imm:
+  (!unaryexp w1. 
+    bir_eval_unaryexp_imm unaryexp (Imm1 w1) (Imm1 ((bir_unaryexp_get_oper unaryexp) w1))) /\
+  (!unaryexp w1. 
+    bir_eval_unaryexp_imm unaryexp (Imm8 w1) (Imm8 ((bir_unaryexp_get_oper unaryexp) w1))) /\
+  (!unaryexp w1. 
+    bir_eval_unaryexp_imm unaryexp (Imm16 w1) (Imm16 ((bir_unaryexp_get_oper unaryexp) w1))) /\
+  (!unaryexp w1. 
+    bir_eval_unaryexp_imm unaryexp (Imm32 w1) (Imm32 ((bir_unaryexp_get_oper unaryexp) w1))) /\
+  (!unaryexp w1. 
+    bir_eval_unaryexp_imm unaryexp (Imm64 w1) (Imm64 ((bir_unaryexp_get_oper unaryexp) w1))) /\
+  (!unaryexp w1. 
+    bir_eval_unaryexp_imm unaryexp (Imm128 w1) (Imm128 ((bir_unaryexp_get_oper unaryexp) w1)))
+End
+
+(* Evaluates a general unary expression with values as parameters *)
+Definition bir_eval_unaryexp_def:
+  (bir_eval_unaryexp unaryexp (BVal_Imm imm1) (BVal_Imm imm) =
+    (bir_eval_unaryexp_imm unaryexp imm1 imm)) /\
+  (bir_eval_unaryexp _ _ _ = F)
+End
+
+(* Gets the operator for a given binary predicate *)
+Definition bir_binpred_get_oper_def:
+  (bir_binpred_get_oper BIExp_Equal = $=) /\
+  (bir_binpred_get_oper BIExp_LessThan = word_lo)
+End
+
+(* Evaluates a binary predicate of two immediates *)
+Inductive bir_eval_binpred_imm:
+  (!binpred w1 w2. 
+    bir_eval_binpred_imm binpred (Imm1 w1) (Imm1 w2) ((bir_binpred_get_oper binpred) w1 w2)) /\
+  (!binpred w1 w2. 
+    bir_eval_binpred_imm binpred (Imm8 w1) (Imm8 w2) ((bir_binpred_get_oper binpred) w1 w2)) /\
+  (!binpred w1 w2. 
+    bir_eval_binpred_imm binpred (Imm16 w1) (Imm16 w2) ((bir_binpred_get_oper binpred) w1 w2)) /\
+  (!binpred w1 w2. 
+    bir_eval_binpred_imm binpred (Imm32 w1) (Imm32 w2) ((bir_binpred_get_oper binpred) w1 w2)) /\
+  (!binpred w1 w2. 
+    bir_eval_binpred_imm binpred (Imm64 w1) (Imm64 w2) ((bir_binpred_get_oper binpred) w1 w2)) /\
+  (!binpred w1 w2. 
+    bir_eval_binpred_imm binpred (Imm128 w1) (Imm128 w2) ((bir_binpred_get_oper binpred) w1 w2))
+End
+
+(* Evaluates a general binary predicate with values as parameters *)
+Inductive bir_eval_binpred:
+  (!binpred imm1 imm2 b. 
+    (bir_eval_binpred_imm binpred imm1 imm2 b) ==>
+    (bir_eval_binpred binpred (BVal_Imm imm1) (BVal_Imm imm2) (BVal_Imm (bool2b b))))
+End
+
+(* Evaluates a general ifthenelse expression with values as parameters *)
+Inductive bir_eval_ifthenelse:
+[~BExp_IfThenElseT:]
+  bir_eval_ifthenelse birT (v1:bir_val_t) (v2:bir_val_t) v1 
+
+[~BExp_IfThenElseF:]
+  bir_eval_ifthenelse birF v1 v2 v2
+End
 
 (* Load a value from the mmap at the given address *)
 Definition bir_load_mmap_def:
@@ -798,7 +442,6 @@ Definition bir_load_mmap_def:
         | NONE => 0
         | SOME v => v
 End
-
 
 (* Concatenate multiple bitstrings to a number on the correct number of bits *)
 Definition bir_mem_concat_def:
@@ -821,7 +464,6 @@ Definition bir_number_of_mem_splits_def:
     else NONE
 End
 
-
 (* Load a bitstring at the given address from a mmap and pad it *)
 Definition bir_load_bitstring_from_mmap_def:
   bir_load_bitstring_from_mmap vty mmap (a:num) =
@@ -833,7 +475,6 @@ Definition bir_load_splits_from_mmap_def:
   bir_load_splits_from_mmap aty vty mmap addr n =
     (MAP (\k. bir_load_bitstring_from_mmap vty mmap (bir_mem_addr aty (addr + k))) (COUNT_LIST n)) 
 End
-
 
 (* Eval an already unpacked load expression *)
 Inductive bir_eval_load_from_mem:
@@ -865,42 +506,12 @@ Definition bir_eval_load_def:
   (bir_eval_load _ _ _ _ _ = F)
 End
 
-(* Computes an already unpacked load expression *)
-Definition bir_compute_load_from_mem_def:
-  bir_compute_load_from_mem
-  (vty : bir_immtype_t) (rty : bir_immtype_t) (aty : bir_immtype_t) (mmap : num |-> num) (en: bir_endian_t) (addr:num) =
-
-   case (bir_number_of_mem_splits vty rty aty) of
-    | NONE => NONE
-    | SOME (n:num) => (
-        let vs = bir_load_splits_from_mmap aty vty mmap addr n in
-        let vs' = (case en of BEnd_LittleEndian => SOME (REVERSE vs)
-                          |  BEnd_BigEndian => SOME vs
-                          |  BEnd_NoEndian => if (n = 1) then SOME vs else NONE) in
-        case vs' of NONE => NONE
-                 |  SOME vs'' => SOME (bir_mem_concat vs'' rty)
-   )
-End
-
-Definition bir_compute_load_def:
-  (bir_compute_load (SOME (BVal_Mem aty vty mmap)) (SOME (BVal_Imm addr)) en rty = 
-    val_from_imm_option (bir_compute_load_from_mem vty rty aty mmap en (b2n addr))) /\
-  (bir_compute_load _ _ _ _ = NONE)
-End
-
-
-(* ----------------------------------------- *)
-(* ----------------- STORE ----------------- *)
-(* ----------------------------------------- *)
-
-
 (* Add all the bitstrings in the mmap at address a *)
 Definition bir_update_mmap_def:
   (bir_update_mmap aty mmap a [] = mmap) /\
   (bir_update_mmap aty mmap a (v::vs) =
     bir_update_mmap aty (FUPDATE mmap ((bir_mem_addr aty a), v2n v)) (SUC a) vs)
 End
-
 
 Inductive bir_eval_store_in_mem:
 [~BEnd_BigEndian:]
@@ -926,7 +537,6 @@ Inductive bir_eval_store_in_mem:
     ==>
     bir_eval_store_in_mem vty aty result mmap BEnd_NoEndian addr
       (BVal_Mem aty vty (bir_update_mmap aty mmap addr ll))
-
 End
 
 Definition bir_eval_store_def:
@@ -934,248 +544,6 @@ Definition bir_eval_store_def:
     bir_eval_store_in_mem vty aty result mmap en (b2n addr) v) /\
   (bir_eval_store _ _ _ _ _ = F)
 End
-
-(* Compute an already unpacked store expression *)
-Definition bir_compute_store_in_mem_def:
-  bir_compute_store_in_mem
-  (vty : bir_immtype_t) (aty : bir_immtype_t) (result : bir_imm_t) (mmap : num |-> num) (en: bir_endian_t) (addr:num) =
-
-   let rty = type_of_bir_imm result in
-   case (bir_number_of_mem_splits vty rty aty) of
-    | NONE => NONE
-    | SOME (n:num) => (
-      case  (bitstring_split (size_of_bir_immtype vty) (b2v result)) of
-        | NONE => NONE
-        | SOME vs =>
-        let vs' = (case en of BEnd_LittleEndian => SOME (REVERSE vs)
-                          |  BEnd_BigEndian => SOME vs
-                          |  BEnd_NoEndian => if (n = 1) then SOME vs else NONE) in
-
-        case vs' of NONE => NONE
-                 |  SOME vs'' => SOME (BVal_Mem aty vty (bir_update_mmap aty mmap addr vs''))
-   )
-End
-
-
-Definition bir_compute_store_def:
-  (bir_compute_store (SOME (BVal_Mem aty vty mmap)) (SOME (BVal_Imm addr)) en (SOME (BVal_Imm result)) = 
-    bir_compute_store_in_mem vty aty result mmap en (b2n addr)) /\
-  (bir_compute_store _ _ _ _ = NONE)
-End
-
-Theorem size_of_bir_immtype_leq_1:
-  !b. 1 <= 2 ** (size_of_bir_immtype b)
-Proof
-  Cases_on `b` >>
-  rw [size_of_bir_immtype_def]
-QED
-
-(* Eval and compute are similar *)
-Theorem bir_eval_load_eq_compute_load:
-  !v_mem v_addr en rty v.
-    bir_eval_load v_mem v_addr en rty v <=>
-    (bir_compute_load (SOME v_mem) (SOME v_addr) en rty = SOME v)
-Proof
-  Cases_on `v_mem` >> Cases_on `v_addr` >> Cases_on `en` >>
-    rw [bir_eval_load_def, bir_eval_load_from_mem_cases] >>
-    rw [bir_compute_load_def, bir_compute_load_from_mem_def] >>
-    CASE_TAC >>
-    simp [] >>
-    rw [val_from_imm_option_def] >>
-    metis_tac []
-QED
-
-
-
-(* If the operands are correctly typed, then the expression evaluates *)
-Theorem type_of_bir_val_imp_bir_eval_load_bigendian:
-  !aty vty v_mem v_addr rty.
-  ((type_of_bir_val v_mem = (BType_Mem aty vty)) /\ 
-    (type_of_bir_val v_addr = BType_Imm aty) /\
-     ((size_of_bir_immtype rty) MOD (size_of_bir_immtype vty) = 0) /\
-     ((size_of_bir_immtype rty) DIV (size_of_bir_immtype vty) <= 
-        2 **(size_of_bir_immtype aty)))
-  ==>
-  ?v. bir_eval_load v_mem v_addr BEnd_BigEndian rty v
-Proof
-  Cases_on `v_mem` >> Cases_on `v_addr` >>
-    rw [bir_eval_load_eq_compute_load] >>
-    rw [bir_compute_load_def, bir_compute_load_from_mem_def, bir_number_of_mem_splits_def] >>
-    fs [type_of_bir_val_def, type_of_bir_imm_def] >>
-    rw [val_from_imm_option_def] >>
-    metis_tac []
-QED
-
-Theorem type_of_bir_val_imp_bir_eval_load_littleendian:
-  !aty vty v_mem v_addr rty.
-  ((type_of_bir_val v_mem = (BType_Mem aty vty)) /\ 
-    (type_of_bir_val v_addr = BType_Imm aty) /\
-     ((size_of_bir_immtype rty) MOD (size_of_bir_immtype vty) = 0) /\
-     ((size_of_bir_immtype rty) DIV (size_of_bir_immtype vty) <= 
-        2 **(size_of_bir_immtype aty)))
-  ==>
-  ?v. bir_eval_load v_mem v_addr BEnd_LittleEndian rty v
-Proof
-  Cases_on `v_mem` >> Cases_on `v_addr` >>
-    rw [bir_eval_load_eq_compute_load] >>
-    rw [bir_compute_load_def, bir_compute_load_from_mem_def, bir_number_of_mem_splits_def] >>
-    fs [type_of_bir_val_def, type_of_bir_imm_def] >>
-    rw [val_from_imm_option_def] >>
-    metis_tac []
-QED
-
-Theorem type_of_bir_val_imp_bir_eval_load_noendian:
-  !aty vty v_mem v_addr rty.
-  ((type_of_bir_val v_mem = (BType_Mem aty vty)) /\ 
-    (type_of_bir_val v_addr = BType_Imm aty) /\
-     ((size_of_bir_immtype rty) MOD (size_of_bir_immtype vty) = 0) /\
-     ((size_of_bir_immtype rty) DIV (size_of_bir_immtype vty) <= 
-        2 **(size_of_bir_immtype aty)) /\
-     ((size_of_bir_immtype rty) DIV (size_of_bir_immtype vty) = 1))
-  ==>
-  ?v. bir_eval_load v_mem v_addr BEnd_NoEndian rty v
-Proof
-  Cases_on `v_mem` >> Cases_on `v_addr` >>
-    rw [bir_eval_load_eq_compute_load] >>
-    rw [bir_compute_load_def, bir_compute_load_from_mem_def, bir_number_of_mem_splits_def] >>
-    fs [type_of_bir_val_def, type_of_bir_imm_def] >>
-    rw [val_from_imm_option_def] >>
-    metis_tac [size_of_bir_immtype_leq_1]
-QED
-
-
-(* Type of bir_mem_concat *)
-Theorem type_of_bir_imm_bir_mem_concat:
-  !vl rty. type_of_bir_imm (bir_mem_concat vl rty) = rty
-Proof
-  Cases_on `rty` >>
-    rw [bir_mem_concat_def, v2bs_def, n2bs_def] >>
-    rw [type_of_bir_imm_def]
-QED
-  
-
-(* Type conservation theorem *)
-Theorem bir_eval_load_correct_type:
-  !v_mem v_addr en rty v.
-    bir_eval_load v_mem v_addr en rty v ==>
-    (type_of_bir_val v = (BType_Imm rty))
-Proof
-  Cases_on `v_mem` >> Cases_on `v_addr` >>
-  Cases_on `en` >>
-
-  simp [bir_eval_load_def, bir_eval_load_from_mem_cases] >>
-  metis_tac [type_of_bir_val_def, type_of_bir_imm_def, type_of_bir_imm_bir_mem_concat]
-QED
-
-(* bitstring_split will never be NONE *)
-Theorem bitstring_split_aux_size_of_bir_immtype:
-  !ty acc bs. ?ll. bitstring_split_aux (size_of_bir_immtype ty) acc bs = SOME ll
-Proof
-  gen_tac >>
-  `?n. size_of_bir_immtype ty = SUC n` by (Cases_on `ty` >> simp [size_of_bir_immtype_def]) >>
-  measureInduct_on `LENGTH bs` >>
-    Cases_on `bs` >>
-    fs [bitstring_split_def, bitstring_split_aux_def] >>
-    `LENGTH (DROP n t) < SUC (LENGTH t)` by rw [listTheory.LENGTH_DROP] >>
-    metis_tac [bitstring_split_aux_def, listTheory.LENGTH_DROP]
-QED
-
-Theorem bitstring_split_size_of_bir_immtype:
-  !ty bs. bitstring_split (size_of_bir_immtype ty) bs <> NONE
-Proof
-  simp [bitstring_split_def] >>
-  metis_tac [bitstring_split_aux_size_of_bir_immtype, optionTheory.NOT_SOME_NONE]
-QED
-
-(* Eval and compute are similar *)
-Theorem bir_eval_store_eq_compute_store:
-  !v_mem v_addr en result v.
-    bir_eval_store v_mem v_addr en result v <=>
-    (bir_compute_store (SOME v_mem) (SOME v_addr) en (SOME result) = SOME v)
-Proof
-  Cases_on `v_mem` >> Cases_on `v_addr` >> Cases_on `en` >> Cases_on `result` >>
-    rw [bir_eval_store_def, bir_eval_store_in_mem_cases] >>
-    rw [bir_compute_store_def, bir_compute_store_in_mem_def] >>
-    CASE_TAC >> CASE_TAC >> TRY CASE_TAC >>
-      simp [] >>
-      metis_tac []
-QED
-
-(* If the operands are correctly typed, then the expression evaluates *)
-Theorem type_of_bir_val_imp_bir_eval_store_bigendian:
-  !aty vty v_mem v_addr v_result rty.
-  ((type_of_bir_val v_mem = (BType_Mem aty vty)) /\ 
-    (type_of_bir_val v_addr = BType_Imm aty) /\
-    (type_of_bir_val v_result = BType_Imm rty) /\
-     ((size_of_bir_immtype rty) MOD (size_of_bir_immtype vty) = 0) /\
-     ((size_of_bir_immtype rty) DIV (size_of_bir_immtype vty) <= 
-        2 **(size_of_bir_immtype aty)))
-  ==>
-  ?v. bir_eval_store v_mem v_addr BEnd_BigEndian v_result v
-Proof
-  Cases_on `v_mem` >> Cases_on `v_addr` >> Cases_on `v_result` >>
-    rw [bir_eval_store_eq_compute_store] >>
-    rw [bir_compute_store_def, bir_compute_store_in_mem_def, bir_number_of_mem_splits_def] >>
-    fs [type_of_bir_val_def, type_of_bir_imm_def] >>
-    TRY CASE_TAC >>
-      fs [bitstring_split_size_of_bir_immtype, bitstring_split_def] >>
-      metis_tac [bitstring_split_aux_size_of_bir_immtype]
-QED
-
-Theorem type_of_bir_val_imp_bir_eval_store_littleendian:
-  !aty vty v_mem v_addr v_result rty.
-  ((type_of_bir_val v_mem = (BType_Mem aty vty)) /\ 
-    (type_of_bir_val v_addr = BType_Imm aty) /\
-    (type_of_bir_val v_result = BType_Imm rty) /\
-     ((size_of_bir_immtype rty) MOD (size_of_bir_immtype vty) = 0) /\
-     ((size_of_bir_immtype rty) DIV (size_of_bir_immtype vty) <= 
-        2 **(size_of_bir_immtype aty)))
-  ==>
-  ?v. bir_eval_store v_mem v_addr BEnd_LittleEndian v_result v
-Proof
-  Cases_on `v_mem` >> Cases_on `v_addr` >> Cases_on `v_result` >>
-    rw [bir_eval_store_eq_compute_store] >>
-    rw [bir_compute_store_def, bir_compute_store_in_mem_def, bir_number_of_mem_splits_def] >>
-    fs [type_of_bir_val_def, type_of_bir_imm_def] >>
-    TRY CASE_TAC >>
-      fs [bitstring_split_size_of_bir_immtype] >>
-      metis_tac []
-QED
-
-Theorem type_of_bir_val_imp_bir_eval_store_noendian:
-  !aty vty v_mem v_addr v_result rty.
-  ((type_of_bir_val v_mem = (BType_Mem aty vty)) /\ 
-    (type_of_bir_val v_addr = BType_Imm aty) /\
-    (type_of_bir_val v_result = BType_Imm rty) /\
-     ((size_of_bir_immtype rty) MOD (size_of_bir_immtype vty) = 0) /\
-     ((size_of_bir_immtype rty) DIV (size_of_bir_immtype vty) <= 
-        2 **(size_of_bir_immtype aty)) /\
-     ((size_of_bir_immtype rty) DIV (size_of_bir_immtype vty) = 1))
-  ==>
-  ?v. bir_eval_store v_mem v_addr BEnd_NoEndian v_result v
-Proof
-  Cases_on `v_mem` >> Cases_on `v_addr` >> Cases_on `v_result` >>
-    rw [bir_eval_store_eq_compute_store] >>
-    rw [bir_compute_store_def, bir_compute_store_in_mem_def, bir_number_of_mem_splits_def] >>
-    fs [type_of_bir_val_def, type_of_bir_imm_def] >>
-    TRY CASE_TAC >>
-      fs [bitstring_split_size_of_bir_immtype] >>
-      metis_tac [size_of_bir_immtype_leq_1]
-QED
-
-(* Type conservation theorem *)
-Theorem bir_eval_store_correct_type:
-  !v_mem v_addr en v_result v.
-    bir_eval_store v_mem v_addr en v_result v ==>
-    (type_of_bir_val v = type_of_bir_val v_mem)
-Proof
-  Cases_on `v_mem` >> Cases_on `v_addr` >> Cases_on `v_result` >>
-  Cases_on `en` >>
-
-  simp [bir_eval_store_def, bir_eval_store_in_mem_cases] >>
-  rw [type_of_bir_val_def, type_of_bir_imm_def] >>
-  metis_tac [type_of_bir_val_def, type_of_bir_imm_def]
-QED
 
 (** definitions *)
 
@@ -1272,6 +640,7 @@ bir_stmt_t =  (* General statement *)
    BStmtB of bir_stmt_basic_t
  | BStmtE of bir_stmt_end_t
 `;
+
 (* Block type : a label, basic statements and an end statement *)
 Datatype:
   bir_block_t = <|
@@ -1297,6 +666,7 @@ bir_status_t =  (* Program state *)
  | BST_Failed (* execution failed *)
  | BST_JumpOutside of bir_label_t (* execution jumped to unknown label *)
 `;
+
 (* Program state *)
 Datatype:
   bir_state_t = <|
